Wolfram: fresh names, non-injective matches, PaperPack sync

RESEARCHER_BUNDLE/artifacts/compiler/ir/HeytingLean/WPP/Wolfram/Hypergraph.c
@@ -1,6 +1,6 @@
 // Lean compiler output
 // Module: HeytingLean.WPP.Wolfram.Hypergraph
-// Imports: Init Mathlib.Data.List.Basic Mathlib.Data.Multiset.MapFold
+// Imports: Init Mathlib.Data.Finset.Basic Mathlib.Data.Finset.Dedup Mathlib.Data.List.Basic Mathlib.Data.Multiset.Basic Mathlib.Data.Multiset.MapFold
 #include <lean/lean.h>
 #if defined(__clang__)
 #pragma clang diagnostic ignored "-Wunused-parameter"
@@ -16,9 +16,16 @@ extern "C" {
 LEAN_EXPORT lean_object* l_HeytingLean_WPP_Wolfram_Expr_rename(lean_object*, lean_object*, lean_object*, lean_object*);
 LEAN_EXPORT lean_object* l_HeytingLean_WPP_Wolfram_Expr_rename___redArg(lean_object*, lean_object*);
 lean_object* l_Multiset_map___redArg(lean_object*, lean_object*);
+LEAN_EXPORT lean_object* l_HeytingLean_WPP_Wolfram_HGraph_verts___redArg(lean_object*, lean_object*);
+LEAN_EXPORT lean_object* l_HeytingLean_WPP_Wolfram_HGraph_verts(lean_object*, lean_object*, lean_object*);
 LEAN_EXPORT lean_object* l_HeytingLean_WPP_Wolfram_HGraph_rename___redArg(lean_object*, lean_object*);
+lean_object* l_List_foldl___redArg(lean_object*, lean_object*, lean_object*);
+lean_object* l_List_dedup___redArg(lean_object*, lean_object*);
 lean_object* l_List_mapTR_loop___at___List_mapAsyncChunked_spec__0___redArg(lean_object*, lean_object*, lean_object*);
+LEAN_EXPORT lean_object* l_HeytingLean_WPP_Wolfram_HGraph_vertsStep(lean_object*, lean_object*, lean_object*, lean_object*);
 LEAN_EXPORT lean_object* l_HeytingLean_WPP_Wolfram_HGraph_rename(lean_object*, lean_object*, lean_object*, lean_object*);
+LEAN_EXPORT lean_object* l_HeytingLean_WPP_Wolfram_HGraph_vertsStep___redArg(lean_object*, lean_object*, lean_object*);
+lean_object* l_Multiset_ndunion___redArg(lean_object*, lean_object*, lean_object*);
 LEAN_EXPORT lean_object* l_HeytingLean_WPP_Wolfram_Expr_rename___redArg(lean_object* x_1, lean_object* x_2) {
 _start:
 {
@@ -56,8 +63,49 @@ x_5 = l_HeytingLean_WPP_Wolfram_HGraph_rename___redArg(x_3, x_4);
 return x_5;
 }
 }
+LEAN_EXPORT lean_object* l_HeytingLean_WPP_Wolfram_HGraph_vertsStep___redArg(lean_object* x_1, lean_object* x_2, lean_object* x_3) {
+_start:
+{
+lean_object* x_4; lean_object* x_5; 
+lean_inc_ref(x_1);
+x_4 = l_List_dedup___redArg(x_1, x_3);
+x_5 = l_Multiset_ndunion___redArg(x_1, x_2, x_4);
+return x_5;
+}
+}
+LEAN_EXPORT lean_object* l_HeytingLean_WPP_Wolfram_HGraph_vertsStep(lean_object* x_1, lean_object* x_2, lean_object* x_3, lean_object* x_4) {
+_start:
+{
+lean_object* x_5; 
+x_5 = l_HeytingLean_WPP_Wolfram_HGraph_vertsStep___redArg(x_2, x_3, x_4);
+return x_5;
+}
+}
+LEAN_EXPORT lean_object* l_HeytingLean_WPP_Wolfram_HGraph_verts___redArg(lean_object* x_1, lean_object* x_2) {
+_start:
+{
+lean_object* x_3; lean_object* x_4; lean_object* x_5; 
+x_3 = lean_alloc_closure((void*)(l_HeytingLean_WPP_Wolfram_HGraph_vertsStep), 4, 2);
+lean_closure_set(x_3, 0, lean_box(0));
+lean_closure_set(x_3, 1, x_1);
+x_4 = lean_box(0);
+x_5 = l_List_foldl___redArg(x_3, x_4, x_2);
+return x_5;
+}
+}
+LEAN_EXPORT lean_object* l_HeytingLean_WPP_Wolfram_HGraph_verts(lean_object* x_1, lean_object* x_2, lean_object* x_3) {
+_start:
+{
+lean_object* x_4; 
+x_4 = l_HeytingLean_WPP_Wolfram_HGraph_verts___redArg(x_2, x_3);
+return x_4;
+}
+}
 lean_object* initialize_Init(uint8_t builtin, lean_object*);
+lean_object* initialize_Mathlib_Data_Finset_Basic(uint8_t builtin, lean_object*);
+lean_object* initialize_Mathlib_Data_Finset_Dedup(uint8_t builtin, lean_object*);
 lean_object* initialize_Mathlib_Data_List_Basic(uint8_t builtin, lean_object*);
+lean_object* initialize_Mathlib_Data_Multiset_Basic(uint8_t builtin, lean_object*);
 lean_object* initialize_Mathlib_Data_Multiset_MapFold(uint8_t builtin, lean_object*);
 static bool _G_initialized = false;
 LEAN_EXPORT lean_object* initialize_HeytingLean_WPP_Wolfram_Hypergraph(uint8_t builtin, lean_object* w) {
@@ -67,7 +115,16 @@ _G_initialized = true;
 res = initialize_Init(builtin, lean_io_mk_world());
 if (lean_io_result_is_error(res)) return res;
 lean_dec_ref(res);
+res = initialize_Mathlib_Data_Finset_Basic(builtin, lean_io_mk_world());
+if (lean_io_result_is_error(res)) return res;
+lean_dec_ref(res);
+res = initialize_Mathlib_Data_Finset_Dedup(builtin, lean_io_mk_world());
+if (lean_io_result_is_error(res)) return res;
+lean_dec_ref(res);
 res = initialize_Mathlib_Data_List_Basic(builtin, lean_io_mk_world());
+if (lean_io_result_is_error(res)) return res;
+lean_dec_ref(res);
+res = initialize_Mathlib_Data_Multiset_Basic(builtin, lean_io_mk_world());
 if (lean_io_result_is_error(res)) return res;
 lean_dec_ref(res);
 res = initialize_Mathlib_Data_Multiset_MapFold(builtin, lean_io_mk_world());
