RESEARCHER_BUNDLE/artifacts/compiler/ir/HeytingLean/WPP/Wolfram/RewriteFresh.c
@@ -1,0 +1,665 @@
+// Lean compiler output
+// Module: HeytingLean.WPP.Wolfram.RewriteFresh
+// Imports: Init Mathlib.Data.Fin.Basic Mathlib.Data.Fintype.Basic Mathlib.Data.Finset.Image Mathlib.Data.List.Nodup Mathlib.Logic.Equiv.Basic Mathlib.Data.Multiset.AddSub HeytingLean.WPP.Wolfram.FreshSupply HeytingLean.WPP.Wolfram.Hypergraph
+#include <lean/lean.h>
+#if defined(__clang__)
+#pragma clang diagnostic ignored "-Wunused-parameter"
+#pragma clang diagnostic ignored "-Wunused-label"
+#elif defined(__GNUC__) && !defined(__CLANG__)
+#pragma GCC diagnostic ignored "-Wunused-parameter"
+#pragma GCC diagnostic ignored "-Wunused-label"
+#pragma GCC diagnostic ignored "-Wunused-but-set-variable"
+#endif
+#ifdef __cplusplus
+extern "C" {
+#endif
+LEAN_EXPORT lean_object* l_HeytingLean_WPP_Wolfram_SystemFresh_Event_swapPerm___redArg(lean_object*, lean_object*, lean_object*, lean_object*);
+LEAN_EXPORT lean_object* l_HeytingLean_WPP_Wolfram_SystemFresh_Event_rule___boxed(lean_object*, lean_object*, lean_object*, lean_object*);
+LEAN_EXPORT lean_object* l_HeytingLean_WPP_Wolfram_SystemFresh_Event_applyWith___redArg(lean_object*, lean_object*, lean_object*, lean_object*, lean_object*);
+LEAN_EXPORT lean_object* l_HeytingLean_WPP_Wolfram_SystemFresh_Event_decidableApplicable___boxed(lean_object*, lean_object*, lean_object*, lean_object*, lean_object*, lean_object*);
+LEAN_EXPORT lean_object* l_HeytingLean_WPP_Wolfram_SystemFresh_Event_instDecidableFreshAssign___boxed(lean_object*, lean_object*, lean_object*, lean_object*, lean_object*, lean_object*, lean_object*);
+uint8_t l_List_decidableSubperm___redArg(lean_object*, lean_object*, lean_object*);
+LEAN_EXPORT lean_object* l_HeytingLean_WPP_Wolfram_SystemFresh_Event_swapPerm___redArg___boxed(lean_object*, lean_object*, lean_object*, lean_object*);
+LEAN_EXPORT lean_object* l_HeytingLean_WPP_Wolfram_SystemFresh_Event_input___boxed(lean_object*, lean_object*, lean_object*, lean_object*);
+lean_object* l_Multiset_map___redArg(lean_object*, lean_object*);
+LEAN_EXPORT uint8_t l_HeytingLean_WPP_Wolfram_SystemFresh_Event_decidableApplicable(lean_object*, lean_object*, lean_object*, lean_object*, lean_object*, lean_object*);
+LEAN_EXPORT lean_object* l_HeytingLean_WPP_Wolfram_RuleFresh_instRhs(lean_object*, lean_object*, lean_object*, lean_object*, lean_object*);
+uint8_t l_Fintype_decidableInjectiveFintype___redArg(lean_object*, lean_object*, lean_object*);
+LEAN_EXPORT uint8_t l_HeytingLean_WPP_Wolfram_SystemFresh_Event_instDecidableFreshAssign___redArg(lean_object*, lean_object*, lean_object*, lean_object*, lean_object*);
+LEAN_EXPORT lean_object* l_HeytingLean_WPP_Wolfram_SystemFresh_Event_rangeFinset___redArg(lean_object*, lean_object*, lean_object*);
+lean_object* l_Equiv_trans___redArg(lean_object*, lean_object*);
+LEAN_EXPORT lean_object* l_HeytingLean_WPP_Wolfram_SystemFresh_Event_input(lean_object*, lean_object*, lean_object*, lean_object*);
+LEAN_EXPORT lean_object* l_HeytingLean_WPP_Wolfram_SystemFresh_Event_instDecidableFreshAssign___redArg___lam__0___boxed(lean_object*, lean_object*, lean_object*, lean_object*);
+LEAN_EXPORT lean_object* l_HeytingLean_WPP_Wolfram_SystemFresh_Event_applyWith___boxed(lean_object*, lean_object*, lean_object*, lean_object*, lean_object*, lean_object*, lean_object*);
+LEAN_EXPORT lean_object* l_HeytingLean_WPP_Wolfram_SystemFresh_Event_swapPerm(lean_object*, lean_object*, lean_object*, lean_object*, lean_object*);
+uint8_t l_List_hasDecEq___redArg(lean_object*, lean_object*, lean_object*);
+LEAN_EXPORT lean_object* l___private_HeytingLean_WPP_Wolfram_RewriteFresh_0__HeytingLean_WPP_Wolfram_SystemFresh_Event_swapPerm_match__1_splitter___redArg___boxed(lean_object*, lean_object*, lean_object*, lean_object*, lean_object*);
+lean_object* l_HeytingLean_WPP_Wolfram_HGraph_verts___redArg(lean_object*, lean_object*);
+static lean_object* l_HeytingLean_WPP_Wolfram_SystemFresh_Event_swapPerm___redArg___closed__0;
+LEAN_EXPORT lean_object* l_HeytingLean_WPP_Wolfram_RuleFresh_instLhs___redArg(lean_object*, lean_object*);
+lean_object* l_HeytingLean_WPP_Wolfram_HGraph_rename___redArg(lean_object*, lean_object*);
+lean_object* l_Multiset_sub___redArg(lean_object*, lean_object*, lean_object*);
+LEAN_EXPORT lean_object* l_HeytingLean_WPP_Wolfram_RuleFresh_instRhs___redArg(lean_object*, lean_object*, lean_object*);
+LEAN_EXPORT lean_object* l_HeytingLean_WPP_Wolfram_SystemFresh_Event_rule(lean_object*, lean_object*, lean_object*, lean_object*);
+LEAN_EXPORT lean_object* l_HeytingLean_WPP_Wolfram_SystemFresh_ctorIdx(lean_object*, lean_object*, lean_object*);
+LEAN_EXPORT lean_object* l_HeytingLean_WPP_Wolfram_SystemFresh_ctorIdx___boxed(lean_object*, lean_object*, lean_object*);
+LEAN_EXPORT uint8_t l_HeytingLean_WPP_Wolfram_SystemFresh_Event_decidableApplicable___redArg___lam__0(lean_object*, lean_object*, lean_object*);
+LEAN_EXPORT lean_object* l_HeytingLean_WPP_Wolfram_SystemFresh_Event_input___redArg(lean_object*, lean_object*);
+LEAN_EXPORT lean_object* l_HeytingLean_WPP_Wolfram_SystemFresh_Event_input___redArg___boxed(lean_object*, lean_object*);
+LEAN_EXPORT lean_object* l_HeytingLean_WPP_Wolfram_RuleFresh_ctorIdx___boxed(lean_object*, lean_object*);
+LEAN_EXPORT uint8_t l_HeytingLean_WPP_Wolfram_SystemFresh_Event_instDecidableFreshAssign___redArg___lam__0(lean_object*, lean_object*, lean_object*, lean_object*);
+LEAN_EXPORT lean_object* l___private_HeytingLean_WPP_Wolfram_RewriteFresh_0__HeytingLean_WPP_Wolfram_SystemFresh_Event_swapPerm_match__1_splitter___redArg(lean_object*, lean_object*, lean_object*, lean_object*, lean_object*);
+lean_object* l_List_appendTR___redArg(lean_object*, lean_object*);
+LEAN_EXPORT lean_object* l_HeytingLean_WPP_Wolfram_RuleFresh_ctorIdx(lean_object*, lean_object*);
+LEAN_EXPORT lean_object* l_HeytingLean_WPP_Wolfram_SystemFresh_Event_instDecidableFreshAssign___redArg___boxed(lean_object*, lean_object*, lean_object*, lean_object*, lean_object*);
+LEAN_EXPORT lean_object* l___private_HeytingLean_WPP_Wolfram_RewriteFresh_0__HeytingLean_WPP_Wolfram_SystemFresh_Event_swapPerm_match__1_splitter(lean_object*, lean_object*, lean_object*, lean_object*, lean_object*, lean_object*, lean_object*);
+LEAN_EXPORT lean_object* l_HeytingLean_WPP_Wolfram_SystemFresh_Event_rangeFinset(lean_object*, lean_object*, lean_object*, lean_object*);
+LEAN_EXPORT lean_object* l_HeytingLean_WPP_Wolfram_SystemFresh_Event_applyWith___redArg___boxed(lean_object*, lean_object*, lean_object*, lean_object*, lean_object*);
+lean_object* l_List_get___redArg(lean_object*, lean_object*);
+uint8_t lean_nat_dec_eq(lean_object*, lean_object*);
+lean_object* lean_nat_mod(lean_object*, lean_object*);
+LEAN_EXPORT lean_object* l_HeytingLean_WPP_Wolfram_SystemFresh_Event_ctorIdx(lean_object*, lean_object*, lean_object*, lean_object*);
+LEAN_EXPORT lean_object* l___private_HeytingLean_WPP_Wolfram_RewriteFresh_0__HeytingLean_WPP_Wolfram_SystemFresh_Event_swapPerm_match__1_splitter___boxed(lean_object*, lean_object*, lean_object*, lean_object*, lean_object*, lean_object*, lean_object*);
+LEAN_EXPORT lean_object* l_HeytingLean_WPP_Wolfram_SystemFresh_Event_ctorIdx___boxed(lean_object*, lean_object*, lean_object*, lean_object*);
+lean_object* l_Fin_succ___redArg(lean_object*);
+uint8_t l_Multiset_decidableMem___redArg(lean_object*, lean_object*, lean_object*);
+LEAN_EXPORT lean_object* l_HeytingLean_WPP_Wolfram_SystemFresh_Event_swapPerm___redArg___lam__0(lean_object*, lean_object*);
+lean_object* l_Equiv_swap___redArg(lean_object*, lean_object*, lean_object*);
+LEAN_EXPORT lean_object* l_HeytingLean_WPP_Wolfram_SystemFresh_Event_rule___redArg(lean_object*, lean_object*);
+LEAN_EXPORT lean_object* l_HeytingLean_WPP_Wolfram_SystemFresh_Event_rule___redArg___boxed(lean_object*, lean_object*);
+lean_object* lean_nat_sub(lean_object*, lean_object*);
+uint8_t l_instDecidableNot___redArg(uint8_t);
+LEAN_EXPORT uint8_t l_HeytingLean_WPP_Wolfram_SystemFresh_Event_decidableApplicable___redArg(lean_object*, lean_object*, lean_object*, lean_object*);
+lean_object* l_List_mapTR(lean_object*, lean_object*, lean_object*, lean_object*);
+LEAN_EXPORT uint8_t l_HeytingLean_WPP_Wolfram_SystemFresh_Event_instDecidableFreshAssign(lean_object*, lean_object*, lean_object*, lean_object*, lean_object*, lean_object*, lean_object*);
+LEAN_EXPORT lean_object* l_HeytingLean_WPP_Wolfram_SystemFresh_Event_swapPerm___redArg___lam__0___boxed(lean_object*, lean_object*);
+lean_object* l_List_finRange(lean_object*);
+lean_object* l_Equiv_refl(lean_object*);
+LEAN_EXPORT lean_object* l_HeytingLean_WPP_Wolfram_SystemFresh_Event_applyWith(lean_object*, lean_object*, lean_object*, lean_object*, lean_object*, lean_object*, lean_object*);
+LEAN_EXPORT lean_object* l_HeytingLean_WPP_Wolfram_SystemFresh_Event_swapPerm___boxed(lean_object*, lean_object*, lean_object*, lean_object*, lean_object*);
+uint8_t l_Nat_decidableForallFin___redArg(lean_object*, lean_object*);
+LEAN_EXPORT lean_object* l_HeytingLean_WPP_Wolfram_SystemFresh_Event_decidableApplicable___redArg___lam__0___boxed(lean_object*, lean_object*, lean_object*);
+lean_object* lean_nat_add(lean_object*, lean_object*);
+lean_object* l_Finset_image___redArg(lean_object*, lean_object*, lean_object*);
+lean_object* l_Sum_elim(lean_object*, lean_object*, lean_object*, lean_object*, lean_object*, lean_object*);
+LEAN_EXPORT lean_object* l_HeytingLean_WPP_Wolfram_RuleFresh_instLhs(lean_object*, lean_object*, lean_object*, lean_object*);
+LEAN_EXPORT lean_object* l_HeytingLean_WPP_Wolfram_SystemFresh_Event_decidableApplicable___redArg___boxed(lean_object*, lean_object*, lean_object*, lean_object*);
+LEAN_EXPORT lean_object* l_HeytingLean_WPP_Wolfram_RuleFresh_ctorIdx(lean_object* x_1, lean_object* x_2) {
+_start:
+{
+lean_object* x_3; 
+x_3 = lean_unsigned_to_nat(0u);
+return x_3;
+}
+}
+LEAN_EXPORT lean_object* l_HeytingLean_WPP_Wolfram_RuleFresh_ctorIdx___boxed(lean_object* x_1, lean_object* x_2) {
+_start:
+{
+lean_object* x_3; 
+x_3 = l_HeytingLean_WPP_Wolfram_RuleFresh_ctorIdx(x_1, x_2);
+lean_dec_ref(x_2);
+return x_3;
+}
+}
+LEAN_EXPORT lean_object* l_HeytingLean_WPP_Wolfram_RuleFresh_instLhs___redArg(lean_object* x_1, lean_object* x_2) {
+_start:
+{
+lean_object* x_3; lean_object* x_4; 
+x_3 = lean_ctor_get(x_1, 1);
+lean_inc(x_3);
+lean_dec_ref(x_1);
+x_4 = l_HeytingLean_WPP_Wolfram_HGraph_rename___redArg(x_2, x_3);
+return x_4;
+}
+}
+LEAN_EXPORT lean_object* l_HeytingLean_WPP_Wolfram_RuleFresh_instLhs(lean_object* x_1, lean_object* x_2, lean_object* x_3, lean_object* x_4) {
+_start:
+{
+lean_object* x_5; 
+x_5 = l_HeytingLean_WPP_Wolfram_RuleFresh_instLhs___redArg(x_3, x_4);
+return x_5;
+}
+}
+LEAN_EXPORT lean_object* l_HeytingLean_WPP_Wolfram_RuleFresh_instRhs___redArg(lean_object* x_1, lean_object* x_2, lean_object* x_3) {
+_start:
+{
+lean_object* x_4; lean_object* x_5; lean_object* x_6; 
+x_4 = lean_ctor_get(x_1, 2);
+lean_inc(x_4);
+lean_dec_ref(x_1);
+x_5 = lean_alloc_closure((void*)(l_Sum_elim), 6, 5);
+lean_closure_set(x_5, 0, lean_box(0));
+lean_closure_set(x_5, 1, lean_box(0));
+lean_closure_set(x_5, 2, lean_box(0));
+lean_closure_set(x_5, 3, x_2);
+lean_closure_set(x_5, 4, x_3);
+x_6 = l_HeytingLean_WPP_Wolfram_HGraph_rename___redArg(x_5, x_4);
+return x_6;
+}
+}
+LEAN_EXPORT lean_object* l_HeytingLean_WPP_Wolfram_RuleFresh_instRhs(lean_object* x_1, lean_object* x_2, lean_object* x_3, lean_object* x_4, lean_object* x_5) {
+_start:
+{
+lean_object* x_6; 
+x_6 = l_HeytingLean_WPP_Wolfram_RuleFresh_instRhs___redArg(x_3, x_4, x_5);
+return x_6;
+}
+}
+LEAN_EXPORT lean_object* l_HeytingLean_WPP_Wolfram_SystemFresh_ctorIdx(lean_object* x_1, lean_object* x_2, lean_object* x_3) {
+_start:
+{
+lean_object* x_4; 
+x_4 = lean_unsigned_to_nat(0u);
+return x_4;
+}
+}
+LEAN_EXPORT lean_object* l_HeytingLean_WPP_Wolfram_SystemFresh_ctorIdx___boxed(lean_object* x_1, lean_object* x_2, lean_object* x_3) {
+_start:
+{
+lean_object* x_4; 
+x_4 = l_HeytingLean_WPP_Wolfram_SystemFresh_ctorIdx(x_1, x_2, x_3);
+lean_dec_ref(x_3);
+return x_4;
+}
+}
+LEAN_EXPORT lean_object* l_HeytingLean_WPP_Wolfram_SystemFresh_Event_ctorIdx(lean_object* x_1, lean_object* x_2, lean_object* x_3, lean_object* x_4) {
+_start:
+{
+lean_object* x_5; 
+x_5 = lean_unsigned_to_nat(0u);
+return x_5;
+}
+}
+LEAN_EXPORT lean_object* l_HeytingLean_WPP_Wolfram_SystemFresh_Event_ctorIdx___boxed(lean_object* x_1, lean_object* x_2, lean_object* x_3, lean_object* x_4) {
+_start:
+{
+lean_object* x_5; 
+x_5 = l_HeytingLean_WPP_Wolfram_SystemFresh_Event_ctorIdx(x_1, x_2, x_3, x_4);
+lean_dec_ref(x_4);
+lean_dec_ref(x_3);
+return x_5;
+}
+}
+LEAN_EXPORT lean_object* l_HeytingLean_WPP_Wolfram_SystemFresh_Event_rule___redArg(lean_object* x_1, lean_object* x_2) {
+_start:
+{
+lean_object* x_3; lean_object* x_4; lean_object* x_5; 
+x_3 = lean_ctor_get(x_1, 0);
+x_4 = lean_ctor_get(x_2, 0);
+lean_inc(x_4);
+lean_dec_ref(x_2);
+x_5 = l_List_get___redArg(x_3, x_4);
+return x_5;
+}
+}
+LEAN_EXPORT lean_object* l_HeytingLean_WPP_Wolfram_SystemFresh_Event_rule(lean_object* x_1, lean_object* x_2, lean_object* x_3, lean_object* x_4) {
+_start:
+{
+lean_object* x_5; 
+x_5 = l_HeytingLean_WPP_Wolfram_SystemFresh_Event_rule___redArg(x_3, x_4);
+return x_5;
+}
+}
+LEAN_EXPORT lean_object* l_HeytingLean_WPP_Wolfram_SystemFresh_Event_rule___redArg___boxed(lean_object* x_1, lean_object* x_2) {
+_start:
+{
+lean_object* x_3; 
+x_3 = l_HeytingLean_WPP_Wolfram_SystemFresh_Event_rule___redArg(x_1, x_2);
+lean_dec_ref(x_1);
+return x_3;
+}
+}
+LEAN_EXPORT lean_object* l_HeytingLean_WPP_Wolfram_SystemFresh_Event_rule___boxed(lean_object* x_1, lean_object* x_2, lean_object* x_3, lean_object* x_4) {
+_start:
+{
+lean_object* x_5; 
+x_5 = l_HeytingLean_WPP_Wolfram_SystemFresh_Event_rule(x_1, x_2, x_3, x_4);
+lean_dec_ref(x_3);
+return x_5;
+}
+}
+LEAN_EXPORT lean_object* l_HeytingLean_WPP_Wolfram_SystemFresh_Event_input___redArg(lean_object* x_1, lean_object* x_2) {
+_start:
+{
+lean_object* x_3; lean_object* x_4; lean_object* x_5; 
+x_3 = lean_ctor_get(x_2, 1);
+lean_inc(x_3);
+x_4 = l_HeytingLean_WPP_Wolfram_SystemFresh_Event_rule___redArg(x_1, x_2);
+x_5 = l_HeytingLean_WPP_Wolfram_RuleFresh_instLhs___redArg(x_4, x_3);
+return x_5;
+}
+}
+LEAN_EXPORT lean_object* l_HeytingLean_WPP_Wolfram_SystemFresh_Event_input(lean_object* x_1, lean_object* x_2, lean_object* x_3, lean_object* x_4) {
+_start:
+{
+lean_object* x_5; 
+x_5 = l_HeytingLean_WPP_Wolfram_SystemFresh_Event_input___redArg(x_3, x_4);
+return x_5;
+}
+}
+LEAN_EXPORT lean_object* l_HeytingLean_WPP_Wolfram_SystemFresh_Event_input___redArg___boxed(lean_object* x_1, lean_object* x_2) {
+_start:
+{
+lean_object* x_3; 
+x_3 = l_HeytingLean_WPP_Wolfram_SystemFresh_Event_input___redArg(x_1, x_2);
+lean_dec_ref(x_1);
+return x_3;
+}
+}
+LEAN_EXPORT lean_object* l_HeytingLean_WPP_Wolfram_SystemFresh_Event_input___boxed(lean_object* x_1, lean_object* x_2, lean_object* x_3, lean_object* x_4) {
+_start:
+{
+lean_object* x_5; 
+x_5 = l_HeytingLean_WPP_Wolfram_SystemFresh_Event_input(x_1, x_2, x_3, x_4);
+lean_dec_ref(x_3);
+return x_5;
+}
+}
+LEAN_EXPORT uint8_t l_HeytingLean_WPP_Wolfram_SystemFresh_Event_instDecidableFreshAssign___redArg___lam__0(lean_object* x_1, lean_object* x_2, lean_object* x_3, lean_object* x_4) {
+_start:
+{
+lean_object* x_5; lean_object* x_6; uint8_t x_7; uint8_t x_8; 
+x_5 = lean_apply_1(x_1, x_4);
+lean_inc_ref(x_2);
+x_6 = l_HeytingLean_WPP_Wolfram_HGraph_verts___redArg(x_2, x_3);
+x_7 = l_Multiset_decidableMem___redArg(x_2, x_5, x_6);
+x_8 = l_instDecidableNot___redArg(x_7);
+return x_8;
+}
+}
+LEAN_EXPORT uint8_t l_HeytingLean_WPP_Wolfram_SystemFresh_Event_instDecidableFreshAssign___redArg(lean_object* x_1, lean_object* x_2, lean_object* x_3, lean_object* x_4, lean_object* x_5) {
+_start:
+{
+lean_object* x_6; lean_object* x_7; lean_object* x_8; lean_object* x_9; lean_object* x_10; uint8_t x_11; 
+x_6 = lean_ctor_get(x_1, 0);
+x_7 = lean_ctor_get(x_3, 0);
+lean_inc(x_7);
+lean_dec_ref(x_3);
+x_8 = l_List_get___redArg(x_6, x_7);
+x_9 = lean_ctor_get(x_8, 0);
+lean_inc(x_9);
+lean_dec_ref(x_8);
+lean_inc(x_9);
+x_10 = l_List_finRange(x_9);
+lean_inc(x_4);
+lean_inc_ref(x_2);
+x_11 = l_Fintype_decidableInjectiveFintype___redArg(x_2, x_10, x_4);
+if (x_11 == 0)
+{
+lean_dec(x_9);
+lean_dec(x_5);
+lean_dec(x_4);
+lean_dec_ref(x_2);
+return x_11;
+}
+else
+{
+lean_object* x_12; uint8_t x_13; 
+x_12 = lean_alloc_closure((void*)(l_HeytingLean_WPP_Wolfram_SystemFresh_Event_instDecidableFreshAssign___redArg___lam__0___boxed), 4, 3);
+lean_closure_set(x_12, 0, x_4);
+lean_closure_set(x_12, 1, x_2);
+lean_closure_set(x_12, 2, x_5);
+x_13 = l_Nat_decidableForallFin___redArg(x_9, x_12);
+lean_dec(x_9);
+return x_13;
+}
+}
+}
+LEAN_EXPORT uint8_t l_HeytingLean_WPP_Wolfram_SystemFresh_Event_instDecidableFreshAssign(lean_object* x_1, lean_object* x_2, lean_object* x_3, lean_object* x_4, lean_object* x_5, lean_object* x_6, lean_object* x_7) {
+_start:
+{
+uint8_t x_8; 
+x_8 = l_HeytingLean_WPP_Wolfram_SystemFresh_Event_instDecidableFreshAssign___redArg(x_3, x_4, x_5, x_6, x_7);
+return x_8;
+}
+}
+LEAN_EXPORT lean_object* l_HeytingLean_WPP_Wolfram_SystemFresh_Event_instDecidableFreshAssign___redArg___lam__0___boxed(lean_object* x_1, lean_object* x_2, lean_object* x_3, lean_object* x_4) {
+_start:
+{
+uint8_t x_5; lean_object* x_6; 
+x_5 = l_HeytingLean_WPP_Wolfram_SystemFresh_Event_instDecidableFreshAssign___redArg___lam__0(x_1, x_2, x_3, x_4);
+x_6 = lean_box(x_5);
+return x_6;
+}
+}
+LEAN_EXPORT lean_object* l_HeytingLean_WPP_Wolfram_SystemFresh_Event_instDecidableFreshAssign___redArg___boxed(lean_object* x_1, lean_object* x_2, lean_object* x_3, lean_object* x_4, lean_object* x_5) {
+_start:
+{
+uint8_t x_6; lean_object* x_7; 
+x_6 = l_HeytingLean_WPP_Wolfram_SystemFresh_Event_instDecidableFreshAssign___redArg(x_1, x_2, x_3, x_4, x_5);
+lean_dec_ref(x_1);
+x_7 = lean_box(x_6);
+return x_7;
+}
+}
+LEAN_EXPORT lean_object* l_HeytingLean_WPP_Wolfram_SystemFresh_Event_instDecidableFreshAssign___boxed(lean_object* x_1, lean_object* x_2, lean_object* x_3, lean_object* x_4, lean_object* x_5, lean_object* x_6, lean_object* x_7) {
+_start:
+{
+uint8_t x_8; lean_object* x_9; 
+x_8 = l_HeytingLean_WPP_Wolfram_SystemFresh_Event_instDecidableFreshAssign(x_1, x_2, x_3, x_4, x_5, x_6, x_7);
+lean_dec_ref(x_3);
+x_9 = lean_box(x_8);
+return x_9;
+}
+}
+LEAN_EXPORT uint8_t l_HeytingLean_WPP_Wolfram_SystemFresh_Event_decidableApplicable___redArg___lam__0(lean_object* x_1, lean_object* x_2, lean_object* x_3) {
+_start:
+{
+uint8_t x_4; 
+x_4 = l_List_hasDecEq___redArg(x_1, x_2, x_3);
+return x_4;
+}
+}
+LEAN_EXPORT uint8_t l_HeytingLean_WPP_Wolfram_SystemFresh_Event_decidableApplicable___redArg(lean_object* x_1, lean_object* x_2, lean_object* x_3, lean_object* x_4) {
+_start:
+{
+lean_object* x_5; lean_object* x_6; lean_object* x_7; lean_object* x_8; lean_object* x_9; lean_object* x_10; lean_object* x_11; lean_object* x_12; uint8_t x_13; 
+x_5 = lean_ctor_get(x_3, 0);
+lean_inc(x_5);
+x_6 = lean_ctor_get(x_3, 1);
+lean_inc(x_6);
+lean_dec_ref(x_3);
+x_7 = lean_ctor_get(x_1, 0);
+x_8 = l_List_get___redArg(x_7, x_5);
+x_9 = lean_ctor_get(x_8, 1);
+lean_inc(x_9);
+lean_dec_ref(x_8);
+x_10 = lean_alloc_closure((void*)(l_HeytingLean_WPP_Wolfram_SystemFresh_Event_decidableApplicable___redArg___lam__0___boxed), 3, 1);
+lean_closure_set(x_10, 0, x_2);
+x_11 = lean_alloc_closure((void*)(l_List_mapTR), 4, 3);
+lean_closure_set(x_11, 0, lean_box(0));
+lean_closure_set(x_11, 1, lean_box(0));
+lean_closure_set(x_11, 2, x_6);
+x_12 = l_Multiset_map___redArg(x_11, x_9);
+x_13 = l_List_decidableSubperm___redArg(x_10, x_12, x_4);
+return x_13;
+}
+}
+LEAN_EXPORT uint8_t l_HeytingLean_WPP_Wolfram_SystemFresh_Event_decidableApplicable(lean_object* x_1, lean_object* x_2, lean_object* x_3, lean_object* x_4, lean_object* x_5, lean_object* x_6) {
+_start:
+{
+uint8_t x_7; 
+x_7 = l_HeytingLean_WPP_Wolfram_SystemFresh_Event_decidableApplicable___redArg(x_3, x_4, x_5, x_6);
+return x_7;
+}
+}
+LEAN_EXPORT lean_object* l_HeytingLean_WPP_Wolfram_SystemFresh_Event_decidableApplicable___redArg___lam__0___boxed(lean_object* x_1, lean_object* x_2, lean_object* x_3) {
+_start:
+{
+uint8_t x_4; lean_object* x_5; 
+x_4 = l_HeytingLean_WPP_Wolfram_SystemFresh_Event_decidableApplicable___redArg___lam__0(x_1, x_2, x_3);
+x_5 = lean_box(x_4);
+return x_5;
+}
+}
+LEAN_EXPORT lean_object* l_HeytingLean_WPP_Wolfram_SystemFresh_Event_decidableApplicable___redArg___boxed(lean_object* x_1, lean_object* x_2, lean_object* x_3, lean_object* x_4) {
+_start:
+{
+uint8_t x_5; lean_object* x_6; 
+x_5 = l_HeytingLean_WPP_Wolfram_SystemFresh_Event_decidableApplicable___redArg(x_1, x_2, x_3, x_4);
+lean_dec_ref(x_1);
+x_6 = lean_box(x_5);
+return x_6;
+}
+}
+LEAN_EXPORT lean_object* l_HeytingLean_WPP_Wolfram_SystemFresh_Event_decidableApplicable___boxed(lean_object* x_1, lean_object* x_2, lean_object* x_3, lean_object* x_4, lean_object* x_5, lean_object* x_6) {
+_start:
+{
+uint8_t x_7; lean_object* x_8; 
+x_7 = l_HeytingLean_WPP_Wolfram_SystemFresh_Event_decidableApplicable(x_1, x_2, x_3, x_4, x_5, x_6);
+lean_dec_ref(x_3);
+x_8 = lean_box(x_7);
+return x_8;
+}
+}
+LEAN_EXPORT lean_object* l_HeytingLean_WPP_Wolfram_SystemFresh_Event_applyWith___redArg(lean_object* x_1, lean_object* x_2, lean_object* x_3, lean_object* x_4, lean_object* x_5) {
+_start:
+{
+lean_object* x_6; lean_object* x_7; lean_object* x_8; lean_object* x_9; lean_object* x_10; lean_object* x_11; lean_object* x_12; 
+x_6 = lean_ctor_get(x_3, 1);
+lean_inc(x_6);
+x_7 = lean_alloc_closure((void*)(l_HeytingLean_WPP_Wolfram_SystemFresh_Event_decidableApplicable___redArg___lam__0___boxed), 3, 1);
+lean_closure_set(x_7, 0, x_2);
+lean_inc_ref(x_3);
+x_8 = l_HeytingLean_WPP_Wolfram_SystemFresh_Event_input___redArg(x_1, x_3);
+x_9 = l_Multiset_sub___redArg(x_7, x_5, x_8);
+x_10 = l_HeytingLean_WPP_Wolfram_SystemFresh_Event_rule___redArg(x_1, x_3);
+x_11 = l_HeytingLean_WPP_Wolfram_RuleFresh_instRhs___redArg(x_10, x_6, x_4);
+x_12 = l_List_appendTR___redArg(x_9, x_11);
+return x_12;
+}
+}
+LEAN_EXPORT lean_object* l_HeytingLean_WPP_Wolfram_SystemFresh_Event_applyWith(lean_object* x_1, lean_object* x_2, lean_object* x_3, lean_object* x_4, lean_object* x_5, lean_object* x_6, lean_object* x_7) {
+_start:
+{
+lean_object* x_8; 
+x_8 = l_HeytingLean_WPP_Wolfram_SystemFresh_Event_applyWith___redArg(x_3, x_4, x_5, x_6, x_7);
+return x_8;
+}
+}
+LEAN_EXPORT lean_object* l_HeytingLean_WPP_Wolfram_SystemFresh_Event_applyWith___redArg___boxed(lean_object* x_1, lean_object* x_2, lean_object* x_3, lean_object* x_4, lean_object* x_5) {
+_start:
+{
+lean_object* x_6; 
+x_6 = l_HeytingLean_WPP_Wolfram_SystemFresh_Event_applyWith___redArg(x_1, x_2, x_3, x_4, x_5);
+lean_dec_ref(x_1);
+return x_6;
+}
+}
+LEAN_EXPORT lean_object* l_HeytingLean_WPP_Wolfram_SystemFresh_Event_applyWith___boxed(lean_object* x_1, lean_object* x_2, lean_object* x_3, lean_object* x_4, lean_object* x_5, lean_object* x_6, lean_object* x_7) {
+_start:
+{
+lean_object* x_8; 
+x_8 = l_HeytingLean_WPP_Wolfram_SystemFresh_Event_applyWith(x_1, x_2, x_3, x_4, x_5, x_6, x_7);
+lean_dec_ref(x_3);
+return x_8;
+}
+}
+LEAN_EXPORT lean_object* l_HeytingLean_WPP_Wolfram_SystemFresh_Event_rangeFinset___redArg(lean_object* x_1, lean_object* x_2, lean_object* x_3) {
+_start:
+{
+lean_object* x_4; lean_object* x_5; 
+x_4 = l_List_finRange(x_2);
+x_5 = l_Finset_image___redArg(x_1, x_3, x_4);
+return x_5;
+}
+}
+LEAN_EXPORT lean_object* l_HeytingLean_WPP_Wolfram_SystemFresh_Event_rangeFinset(lean_object* x_1, lean_object* x_2, lean_object* x_3, lean_object* x_4) {
+_start:
+{
+lean_object* x_5; 
+x_5 = l_HeytingLean_WPP_Wolfram_SystemFresh_Event_rangeFinset___redArg(x_2, x_3, x_4);
+return x_5;
+}
+}
+LEAN_EXPORT lean_object* l_HeytingLean_WPP_Wolfram_SystemFresh_Event_swapPerm___redArg___lam__0(lean_object* x_1, lean_object* x_2) {
+_start:
+{
+lean_object* x_3; lean_object* x_4; 
+x_3 = l_Fin_succ___redArg(x_2);
+x_4 = lean_apply_1(x_1, x_3);
+return x_4;
+}
+}
+static lean_object* _init_l_HeytingLean_WPP_Wolfram_SystemFresh_Event_swapPerm___redArg___closed__0() {
+_start:
+{
+lean_object* x_1; 
+x_1 = l_Equiv_refl(lean_box(0));
+return x_1;
+}
+}
+LEAN_EXPORT lean_object* l_HeytingLean_WPP_Wolfram_SystemFresh_Event_swapPerm___redArg(lean_object* x_1, lean_object* x_2, lean_object* x_3, lean_object* x_4) {
+_start:
+{
+lean_object* x_5; uint8_t x_6; 
+x_5 = lean_unsigned_to_nat(0u);
+x_6 = lean_nat_dec_eq(x_2, x_5);
+if (x_6 == 1)
+{
+lean_object* x_7; 
+lean_dec(x_4);
+lean_dec(x_3);
+lean_dec_ref(x_1);
+x_7 = l_HeytingLean_WPP_Wolfram_SystemFresh_Event_swapPerm___redArg___closed__0;
+return x_7;
+}
+else
+{
+lean_object* x_8; lean_object* x_9; lean_object* x_10; lean_object* x_11; lean_object* x_12; lean_object* x_13; lean_object* x_14; lean_object* x_15; lean_object* x_16; lean_object* x_17; lean_object* x_18; 
+lean_inc(x_4);
+x_8 = lean_alloc_closure((void*)(l_HeytingLean_WPP_Wolfram_SystemFresh_Event_swapPerm___redArg___lam__0___boxed), 2, 1);
+lean_closure_set(x_8, 0, x_4);
+lean_inc(x_3);
+x_9 = lean_alloc_closure((void*)(l_HeytingLean_WPP_Wolfram_SystemFresh_Event_swapPerm___redArg___lam__0___boxed), 2, 1);
+lean_closure_set(x_9, 0, x_3);
+x_10 = lean_unsigned_to_nat(1u);
+x_11 = lean_nat_sub(x_2, x_10);
+x_12 = lean_nat_add(x_11, x_10);
+x_13 = lean_nat_mod(x_5, x_12);
+lean_dec(x_12);
+lean_inc(x_13);
+x_14 = lean_apply_1(x_3, x_13);
+x_15 = lean_apply_1(x_4, x_13);
+lean_inc_ref(x_1);
+x_16 = l_Equiv_swap___redArg(x_1, x_14, x_15);
+x_17 = l_HeytingLean_WPP_Wolfram_SystemFresh_Event_swapPerm___redArg(x_1, x_11, x_9, x_8);
+lean_dec(x_11);
+x_18 = l_Equiv_trans___redArg(x_16, x_17);
+return x_18;
+}
+}
+}
+LEAN_EXPORT lean_object* l_HeytingLean_WPP_Wolfram_SystemFresh_Event_swapPerm(lean_object* x_1, lean_object* x_2, lean_object* x_3, lean_object* x_4, lean_object* x_5) {
+_start:
+{
+lean_object* x_6; 
+x_6 = l_HeytingLean_WPP_Wolfram_SystemFresh_Event_swapPerm___redArg(x_2, x_3, x_4, x_5);
+return x_6;
+}
+}
+LEAN_EXPORT lean_object* l_HeytingLean_WPP_Wolfram_SystemFresh_Event_swapPerm___redArg___lam__0___boxed(lean_object* x_1, lean_object* x_2) {
+_start:
+{
+lean_object* x_3; 
+x_3 = l_HeytingLean_WPP_Wolfram_SystemFresh_Event_swapPerm___redArg___lam__0(x_1, x_2);
+lean_dec(x_2);
+return x_3;
+}
+}
+LEAN_EXPORT lean_object* l_HeytingLean_WPP_Wolfram_SystemFresh_Event_swapPerm___redArg___boxed(lean_object* x_1, lean_object* x_2, lean_object* x_3, lean_object* x_4) {
+_start:
+{
+lean_object* x_5; 
+x_5 = l_HeytingLean_WPP_Wolfram_SystemFresh_Event_swapPerm___redArg(x_1, x_2, x_3, x_4);
+lean_dec(x_2);
+return x_5;
+}
+}
+LEAN_EXPORT lean_object* l_HeytingLean_WPP_Wolfram_SystemFresh_Event_swapPerm___boxed(lean_object* x_1, lean_object* x_2, lean_object* x_3, lean_object* x_4, lean_object* x_5) {
+_start:
+{
+lean_object* x_6; 
+x_6 = l_HeytingLean_WPP_Wolfram_SystemFresh_Event_swapPerm(x_1, x_2, x_3, x_4, x_5);
+lean_dec(x_3);
+return x_6;
+}
+}
+LEAN_EXPORT lean_object* l___private_HeytingLean_WPP_Wolfram_RewriteFresh_0__HeytingLean_WPP_Wolfram_SystemFresh_Event_swapPerm_match__1_splitter___redArg(lean_object* x_1, lean_object* x_2, lean_object* x_3, lean_object* x_4, lean_object* x_5) {
+_start:
+{
+lean_object* x_6; uint8_t x_7; 
+x_6 = lean_unsigned_to_nat(0u);
+x_7 = lean_nat_dec_eq(x_1, x_6);
+if (x_7 == 1)
+{
+lean_object* x_8; 
+lean_dec(x_5);
+x_8 = lean_apply_2(x_4, x_2, x_3);
+return x_8;
+}
+else
+{
+lean_object* x_9; lean_object* x_10; lean_object* x_11; 
+lean_dec(x_4);
+x_9 = lean_unsigned_to_nat(1u);
+x_10 = lean_nat_sub(x_1, x_9);
+x_11 = lean_apply_3(x_5, x_10, x_2, x_3);
+return x_11;
+}
+}
+}
+LEAN_EXPORT lean_object* l___private_HeytingLean_WPP_Wolfram_RewriteFresh_0__HeytingLean_WPP_Wolfram_SystemFresh_Event_swapPerm_match__1_splitter(lean_object* x_1, lean_object* x_2, lean_object* x_3, lean_object* x_4, lean_object* x_5, lean_object* x_6, lean_object* x_7) {
+_start:
+{
+lean_object* x_8; 
+x_8 = l___private_HeytingLean_WPP_Wolfram_RewriteFresh_0__HeytingLean_WPP_Wolfram_SystemFresh_Event_swapPerm_match__1_splitter___redArg(x_3, x_4, x_5, x_6, x_7);
+return x_8;
+}
+}
+LEAN_EXPORT lean_object* l___private_HeytingLean_WPP_Wolfram_RewriteFresh_0__HeytingLean_WPP_Wolfram_SystemFresh_Event_swapPerm_match__1_splitter___redArg___boxed(lean_object* x_1, lean_object* x_2, lean_object* x_3, lean_object* x_4, lean_object* x_5) {
+_start:
+{
+lean_object* x_6; 
+x_6 = l___private_HeytingLean_WPP_Wolfram_RewriteFresh_0__HeytingLean_WPP_Wolfram_SystemFresh_Event_swapPerm_match__1_splitter___redArg(x_1, x_2, x_3, x_4, x_5);
+lean_dec(x_1);
+return x_6;
+}
+}
+LEAN_EXPORT lean_object* l___private_HeytingLean_WPP_Wolfram_RewriteFresh_0__HeytingLean_WPP_Wolfram_SystemFresh_Event_swapPerm_match__1_splitter___boxed(lean_object* x_1, lean_object* x_2, lean_object* x_3, lean_object* x_4, lean_object* x_5, lean_object* x_6, lean_object* x_7) {
+_start:
+{
+lean_object* x_8; 
+x_8 = l___private_HeytingLean_WPP_Wolfram_RewriteFresh_0__HeytingLean_WPP_Wolfram_SystemFresh_Event_swapPerm_match__1_splitter(x_1, x_2, x_3, x_4, x_5, x_6, x_7);
+lean_dec(x_3);
+return x_8;
+}
+}
+lean_object* initialize_Init(uint8_t builtin, lean_object*);
+lean_object* initialize_Mathlib_Data_Fin_Basic(uint8_t builtin, lean_object*);
+lean_object* initialize_Mathlib_Data_Fintype_Basic(uint8_t builtin, lean_object*);
+lean_object* initialize_Mathlib_Data_Finset_Image(uint8_t builtin, lean_object*);
+lean_object* initialize_Mathlib_Data_List_Nodup(uint8_t builtin, lean_object*);
+lean_object* initialize_Mathlib_Logic_Equiv_Basic(uint8_t builtin, lean_object*);
+lean_object* initialize_Mathlib_Data_Multiset_AddSub(uint8_t builtin, lean_object*);
+lean_object* initialize_HeytingLean_WPP_Wolfram_FreshSupply(uint8_t builtin, lean_object*);
+lean_object* initialize_HeytingLean_WPP_Wolfram_Hypergraph(uint8_t builtin, lean_object*);
+static bool _G_initialized = false;
+LEAN_EXPORT lean_object* initialize_HeytingLean_WPP_Wolfram_RewriteFresh(uint8_t builtin, lean_object* w) {
+lean_object * res;
+if (_G_initialized) return lean_io_result_mk_ok(lean_box(0));
+_G_initialized = true;
+res = initialize_Init(builtin, lean_io_mk_world());
+if (lean_io_result_is_error(res)) return res;
+lean_dec_ref(res);
+res = initialize_Mathlib_Data_Fin_Basic(builtin, lean_io_mk_world());
+if (lean_io_result_is_error(res)) return res;
+lean_dec_ref(res);
+res = initialize_Mathlib_Data_Fintype_Basic(builtin, lean_io_mk_world());
+if (lean_io_result_is_error(res)) return res;
+lean_dec_ref(res);
+res = initialize_Mathlib_Data_Finset_Image(builtin, lean_io_mk_world());
+if (lean_io_result_is_error(res)) return res;
+lean_dec_ref(res);
+res = initialize_Mathlib_Data_List_Nodup(builtin, lean_io_mk_world());
+if (lean_io_result_is_error(res)) return res;
+lean_dec_ref(res);
+res = initialize_Mathlib_Logic_Equiv_Basic(builtin, lean_io_mk_world());
+if (lean_io_result_is_error(res)) return res;
+lean_dec_ref(res);
+res = initialize_Mathlib_Data_Multiset_AddSub(builtin, lean_io_mk_world());
+if (lean_io_result_is_error(res)) return res;
+lean_dec_ref(res);
+res = initialize_HeytingLean_WPP_Wolfram_FreshSupply(builtin, lean_io_mk_world());
+if (lean_io_result_is_error(res)) return res;
+lean_dec_ref(res);
+res = initialize_HeytingLean_WPP_Wolfram_Hypergraph(builtin, lean_io_mk_world());
+if (lean_io_result_is_error(res)) return res;
+lean_dec_ref(res);
+l_HeytingLean_WPP_Wolfram_SystemFresh_Event_swapPerm___redArg___closed__0 = _init_l_HeytingLean_WPP_Wolfram_SystemFresh_Event_swapPerm___redArg___closed__0();
+lean_mark_persistent(l_HeytingLean_WPP_Wolfram_SystemFresh_Event_swapPerm___redArg___closed__0);
+return lean_io_result_mk_ok(lean_box(0));
+}
+#ifdef __cplusplus
+}
+#endif
